WIP

Engine/Meta/Meta.v
@@ -12,15 +12,130 @@ Require Import List.
 Import ListNotations.
 
 From Linden Require Import Regex Chars Semantics Tree.
-From Linden Require Import FunctionalUtils.
 From Linden Require Import Parameters LWParameters.
-From Linden Require Import StrictSuffix Prefix.
-From Linden Require Import EngineSpec MetaLiterals.
+From Linden Require Import Prefix.
+From Linden Require Import EngineSpec MetaLiterals MetaAnchored.
+From Linden Require Import PikeSubset SeenSets.
+From Linden Require Import Tactics.
 From Warblre Require Import Base RegExpRecord.
 
 
 Section Meta.
   Context {params: LindenParameters}.
   Context (rer: RegExpRecord).
+
+Definition meta_supported_regex (r:regex) : bool :=
+  is_pike_regex r.
+
+(* The configuration of a Meta engine search *)
+Record meta_config := {
+  (* the memory limit the search should try to respect *)
+  (* expressed in a somewhat arbitrary unit, attemps to be the unit of a pointer size *)
+  (* if not specified, there is no limit *)
+  memory_limit : option nat;
+}.
+
+(* FIXME: move this computation to FunctionalMemoBT and it should be with regards to :code, not regex size *)
+Definition memobt_peak_memory_usage (r:regex) (inp:input) : nat :=
+  regex_size r * total_length inp.
+
+(* an anchored search with heuristics *)
+Definition meta_search_anchored (config:meta_config) (r:regex) (inp:input) : option leaf :=
+  let can_use_memobt := match config.(memory_limit) with
+    | Some lim => memobt_peak_memory_usage r inp <=? lim
+    | None => true
+  end in
+  if can_use_memobt then
+    (* FIXME: how come we do not need to provide the MemoSet instance? *)
+    @exec _ _ (@MemoBTAnchoredEngine _ rer) r inp
+  else
+    @exec _ _ (@PikeVMAnchoredEngine VMSlist _ rer BruteForceStrSearch) r inp.
+
+Theorem meta_search_anchored_correct (config:meta_config):
+  forall r inp tree,
+    meta_supported_regex r = true ->
+    is_tree rer [Areg r] inp Groups.GroupMap.empty forward tree ->
+    first_leaf tree inp = meta_search_anchored config r inp.
+Proof.
+  intros r inp tree Hsup Htree.
+  unfold meta_search_anchored.
+  case_if.
+  - eapply exec_correct; eauto.
+    (* FIXME: we forgot that the supported regex is the one from pikevm? *)
+    admit.
+  - eapply exec_correct; eauto.
+    (* FIXME: we forgot that the supported regex is the one from pikevm? *)
+    admit.
+Admitted.
+
+Instance MetaSearchAnchored (config:meta_config): AnchoredEngine rer := {
+  exec := meta_search_anchored config;
+  supported_regex := meta_supported_regex;
+  exec_correct := meta_search_anchored_correct config
+}.
+
+(* MemoBT supports lazy_prefix *)
+Lemma lazy_prefix_supported_memobt:
+  @lazy_prefix_supported _ rer (MemoBTAnchoredEngine rer).
+Proof.
+  intros r Hsup.
+  (* FIXME: we forgot that the supported regex is the one from memobt? *)
+  admit.
+Admitted.
+
+(* FIXME: support the MemoBT *)
+Definition search (config:meta_config) (r:regex) (inp:input) : option leaf :=
+  match @try_lit_search _ rer BruteForceStrSearch r inp with
+  | Some ol => ol
+  | None =>
+    match @try_anchored_search _ _ (@MetaSearchAnchored config) r inp with
+    | Some ol => ol
+    | None =>
+        let can_use_memobt := match config.(memory_limit) with
+          | Some lim => memobt_peak_memory_usage r inp <=? lim
+          | None => true
+        end in
+        if can_use_memobt then
+          @un_exec _ _ (@UnanchorEngine _ rer (@MemoBTAnchoredEngine _ rer) lazy_prefix_supported_memobt) r inp
+        else
+          @un_exec _ _ (@PikeVMUnanchoredEngine VMSlist _ rer BruteForceStrSearch) r inp
+    end
+  end.
+
+
+Theorem search_correct (config:meta_config):
+  forall r inp tree,
+    meta_supported_regex r = true ->
+    is_tree rer [Areg (lazy_prefix r)] inp Groups.GroupMap.empty forward tree ->
+    first_leaf tree inp = search config r inp.
+Proof.
+  intros r inp tree Hsup Htree.
+  unfold search.
+  unfold meta_supported_regex in Hsup.
+  destruct try_lit_search as [ol'|] eqn:Hlit.
+  - (* literal search succeeded *)
+    eapply try_lit_search_correct in Hlit; eauto.
+  - (* literal search failed, try anchored search *)
+    destruct try_anchored_search as [ol'|] eqn:Hanch.
+    + (* anchored search succeeded *)
+      eapply try_anchored_search_correct in Hanch as <-; eauto.
+    + (* anchored search not applicable, fall back to unanchored search *)
+      case_if.
+      * (* use tha MemoBT engine *)
+        eapply un_exec_correct; eauto.
+        (* FIXME: we forgot that the supported regex is the one from pikevm? *)
+        admit.
+      * (* use tha PikeVM engine *)
+        eapply un_exec_correct; eauto.
+        (* FIXME: we forgot that the supported regex is the one from pikevm? *)
+        admit.
+Admitted.
+
+
+Instance MetaEngine (config:meta_config): UnanchoredEngine rer := {
+  un_exec := search config;
+  un_supported_regex := meta_supported_regex;
+  un_exec_correct := search_correct config
+}.
 
 End Meta.
